tests/fstar/hashmap/Hashmap.Funs.fst
@@ -11,7 +11,7 @@ include Hashmap.Clauses
 let hash_key (k : usize) : result usize =
   Return k
 
-(** [hashmap::HashMap::{0}::allocate_slots]: loop 0: forward function *)
+(** [hashmap::{hashmap::HashMap<T>}::allocate_slots]: loop 0: forward function *)
 let rec hashMap_allocate_slots_loop
   (t : Type0) (slots : alloc_vec_Vec (list_t t)) (n : usize) :
   Tot (result (alloc_vec_Vec (list_t t)))
@@ -24,14 +24,14 @@ let rec hashMap_allocate_slots_loop
     hashMap_allocate_slots_loop t slots0 n0
   else Return slots
 
-(** [hashmap::HashMap::{0}::allocate_slots]: forward function *)
+(** [hashmap::{hashmap::HashMap<T>}::allocate_slots]: forward function *)
 let hashMap_allocate_slots
   (t : Type0) (slots : alloc_vec_Vec (list_t t)) (n : usize) :
   result (alloc_vec_Vec (list_t t))
   =
   hashMap_allocate_slots_loop t slots n
 
-(** [hashmap::HashMap::{0}::new_with_capacity]: forward function *)
+(** [hashmap::{hashmap::HashMap<T>}::new_with_capacity]: forward function *)
 let hashMap_new_with_capacity
   (t : Type0) (capacity : usize) (max_load_dividend : usize)
   (max_load_divisor : usize) :
@@ -49,11 +49,11 @@ let hashMap_new_with_capacity
       slots = slots
     }
 
-(** [hashmap::HashMap::{0}::new]: forward function *)
+(** [hashmap::{hashmap::HashMap<T>}::new]: forward function *)
 let hashMap_new (t : Type0) : result (hashMap_t t) =
   hashMap_new_with_capacity t 32 4 5
 
-(** [hashmap::HashMap::{0}::clear]: loop 0: merged forward/backward function
+(** [hashmap::{hashmap::HashMap<T>}::clear]: loop 0: merged forward/backward function
     (there is a single backward function, and the forward function returns ()) *)
 let rec hashMap_clear_loop
   (t : Type0) (slots : alloc_vec_Vec (list_t t)) (i : usize) :
@@ -66,22 +66,22 @@ let rec hashMap_clear_loop
     let* i1 = usize_add i 1 in
     let* slots0 =
       alloc_vec_Vec_index_mut_back (list_t t) usize
-        (core_slice_index_usize_coresliceindexSliceIndexInst (list_t t)) slots
-        i List_Nil in
+        (core_slice_index_SliceIndexUsizeSliceTInst (list_t t)) slots i
+        List_Nil in
     hashMap_clear_loop t slots0 i1
   else Return slots
 
-(** [hashmap::HashMap::{0}::clear]: merged forward/backward function
+(** [hashmap::{hashmap::HashMap<T>}::clear]: merged forward/backward function
     (there is a single backward function, and the forward function returns ()) *)
 let hashMap_clear (t : Type0) (self : hashMap_t t) : result (hashMap_t t) =
   let* v = hashMap_clear_loop t self.slots 0 in
   Return { self with num_entries = 0; slots = v }
 
-(** [hashmap::HashMap::{0}::len]: forward function *)
+(** [hashmap::{hashmap::HashMap<T>}::len]: forward function *)
 let hashMap_len (t : Type0) (self : hashMap_t t) : result usize =
   Return self.num_entries
 
-(** [hashmap::HashMap::{0}::insert_in_list]: loop 0: forward function *)
+(** [hashmap::{hashmap::HashMap<T>}::insert_in_list]: loop 0: forward function *)
 let rec hashMap_insert_in_list_loop
   (t : Type0) (key : usize) (value : t) (ls : list_t t) :
   Tot (result bool)
@@ -95,12 +95,12 @@ let rec hashMap_insert_in_list_loop
   | List_Nil -> Return true
   end
 
-(** [hashmap::HashMap::{0}::insert_in_list]: forward function *)
+(** [hashmap::{hashmap::HashMap<T>}::insert_in_list]: forward function *)
 let hashMap_insert_in_list
   (t : Type0) (key : usize) (value : t) (ls : list_t t) : result bool =
   hashMap_insert_in_list_loop t key value ls
 
-(** [hashmap::HashMap::{0}::insert_in_list]: loop 0: backward function 0 *)
+(** [hashmap::{hashmap::HashMap<T>}::insert_in_list]: loop 0: backward function 0 *)
 let rec hashMap_insert_in_list_loop_back
   (t : Type0) (key : usize) (value : t) (ls : list_t t) :
   Tot (result (list_t t))
@@ -116,12 +116,12 @@ let rec hashMap_insert_in_list_loop_back
   | List_Nil -> let l = List_Nil in Return (List_Cons key value l)
   end
 
-(** [hashmap::HashMap::{0}::insert_in_list]: backward function 0 *)
+(** [hashmap::{hashmap::HashMap<T>}::insert_in_list]: backward function 0 *)
 let hashMap_insert_in_list_back
   (t : Type0) (key : usize) (value : t) (ls : list_t t) : result (list_t t) =
   hashMap_insert_in_list_loop_back t key value ls
 
-(** [hashmap::HashMap::{0}::insert_no_resize]: merged forward/backward function
+(** [hashmap::{hashmap::HashMap<T>}::insert_no_resize]: merged forward/backward function
     (there is a single backward function, and the forward function returns ()) *)
 let hashMap_insert_no_resize
   (t : Type0) (self : hashMap_t t) (key : usize) (value : t) :
@@ -132,8 +132,8 @@ let hashMap_insert_no_resize
   let* hash_mod = usize_rem hash i in
   let* l =
     alloc_vec_Vec_index_mut (list_t t) usize
-      (core_slice_index_usize_coresliceindexSliceIndexInst (list_t t))
-      self.slots hash_mod in
+      (core_slice_index_SliceIndexUsizeSliceTInst (list_t t)) self.slots
+      hash_mod in
   let* inserted = hashMap_insert_in_list t key value l in
   if inserted
   then
@@ -141,18 +141,18 @@ let hashMap_insert_no_resize
     let* l0 = hashMap_insert_in_list_back t key value l in
     let* v =
       alloc_vec_Vec_index_mut_back (list_t t) usize
-        (core_slice_index_usize_coresliceindexSliceIndexInst (list_t t))
-        self.slots hash_mod l0 in
+        (core_slice_index_SliceIndexUsizeSliceTInst (list_t t)) self.slots
+        hash_mod l0 in
     Return { self with num_entries = i0; slots = v }
   else
     let* l0 = hashMap_insert_in_list_back t key value l in
     let* v =
       alloc_vec_Vec_index_mut_back (list_t t) usize
-        (core_slice_index_usize_coresliceindexSliceIndexInst (list_t t))
-        self.slots hash_mod l0 in
+        (core_slice_index_SliceIndexUsizeSliceTInst (list_t t)) self.slots
+        hash_mod l0 in
     Return { self with slots = v }
 
-(** [hashmap::HashMap::{0}::move_elements_from_list]: loop 0: merged forward/backward function
+(** [hashmap::{hashmap::HashMap<T>}::move_elements_from_list]: loop 0: merged forward/backward function
     (there is a single backward function, and the forward function returns ()) *)
 let rec hashMap_move_elements_from_list_loop
   (t : Type0) (ntable : hashMap_t t) (ls : list_t t) :
@@ -166,13 +166,13 @@ let rec hashMap_move_elements_from_list_loop
   | List_Nil -> Return ntable
   end
 
-(** [hashmap::HashMap::{0}::move_elements_from_list]: merged forward/backward function
+(** [hashmap::{hashmap::HashMap<T>}::move_elements_from_list]: merged forward/backward function
     (there is a single backward function, and the forward function returns ()) *)
 let hashMap_move_elements_from_list
   (t : Type0) (ntable : hashMap_t t) (ls : list_t t) : result (hashMap_t t) =
   hashMap_move_elements_from_list_loop t ntable ls
 
-(** [hashmap::HashMap::{0}::move_elements]: loop 0: merged forward/backward function
+(** [hashmap::{hashmap::HashMap<T>}::move_elements]: loop 0: merged forward/backward function
     (there is a single backward function, and the forward function returns ()) *)
 let rec hashMap_move_elements_loop
   (t : Type0) (ntable : hashMap_t t) (slots : alloc_vec_Vec (list_t t))
@@ -185,20 +185,18 @@ let rec hashMap_move_elements_loop
   then
     let* l =
       alloc_vec_Vec_index_mut (list_t t) usize
-        (core_slice_index_usize_coresliceindexSliceIndexInst (list_t t)) slots
-        i in
+        (core_slice_index_SliceIndexUsizeSliceTInst (list_t t)) slots i in
     let ls = core_mem_replace (list_t t) l List_Nil in
     let* ntable0 = hashMap_move_elements_from_list t ntable ls in
     let* i1 = usize_add i 1 in
     let l0 = core_mem_replace_back (list_t t) l List_Nil in
     let* slots0 =
       alloc_vec_Vec_index_mut_back (list_t t) usize
-        (core_slice_index_usize_coresliceindexSliceIndexInst (list_t t)) slots
-        i l0 in
+        (core_slice_index_SliceIndexUsizeSliceTInst (list_t t)) slots i l0 in
     hashMap_move_elements_loop t ntable0 slots0 i1
   else Return (ntable, slots)
 
-(** [hashmap::HashMap::{0}::move_elements]: merged forward/backward function
+(** [hashmap::{hashmap::HashMap<T>}::move_elements]: merged forward/backward function
     (there is a single backward function, and the forward function returns ()) *)
 let hashMap_move_elements
   (t : Type0) (ntable : hashMap_t t) (slots : alloc_vec_Vec (list_t t))
@@ -207,7 +205,7 @@ let hashMap_move_elements
   =
   hashMap_move_elements_loop t ntable slots i
 
-(** [hashmap::HashMap::{0}::try_resize]: merged forward/backward function
+(** [hashmap::{hashmap::HashMap<T>}::try_resize]: merged forward/backward function
     (there is a single backward function, and the forward function returns ()) *)
 let hashMap_try_resize
   (t : Type0) (self : hashMap_t t) : result (hashMap_t t) =
@@ -226,7 +224,7 @@ let hashMap_try_resize
       }
   else Return { self with max_load_factor = (i, i0) }
 
-(** [hashmap::HashMap::{0}::insert]: merged forward/backward function
+(** [hashmap::{hashmap::HashMap<T>}::insert]: merged forward/backward function
     (there is a single backward function, and the forward function returns ()) *)
 let hashMap_insert
   (t : Type0) (self : hashMap_t t) (key : usize) (value : t) :
@@ -236,7 +234,7 @@ let hashMap_insert
   let* i = hashMap_len t self0 in
   if i > self0.max_load then hashMap_try_resize t self0 else Return self0
 
-(** [hashmap::HashMap::{0}::contains_key_in_list]: loop 0: forward function *)
+(** [hashmap::{hashmap::HashMap<T>}::contains_key_in_list]: loop 0: forward function *)
 let rec hashMap_contains_key_in_list_loop
   (t : Type0) (key : usize) (ls : list_t t) :
   Tot (result bool)
@@ -250,12 +248,12 @@ let rec hashMap_contains_key_in_list_loop
   | List_Nil -> Return false
   end
 
-(** [hashmap::HashMap::{0}::contains_key_in_list]: forward function *)
+(** [hashmap::{hashmap::HashMap<T>}::contains_key_in_list]: forward function *)
 let hashMap_contains_key_in_list
   (t : Type0) (key : usize) (ls : list_t t) : result bool =
   hashMap_contains_key_in_list_loop t key ls
 
-(** [hashmap::HashMap::{0}::contains_key]: forward function *)
+(** [hashmap::{hashmap::HashMap<T>}::contains_key]: forward function *)
 let hashMap_contains_key
   (t : Type0) (self : hashMap_t t) (key : usize) : result bool =
   let* hash = hash_key key in
@@ -263,11 +261,11 @@ let hashMap_contains_key
   let* hash_mod = usize_rem hash i in
   let* l =
     alloc_vec_Vec_index (list_t t) usize
-      (core_slice_index_usize_coresliceindexSliceIndexInst (list_t t))
-      self.slots hash_mod in
+      (core_slice_index_SliceIndexUsizeSliceTInst (list_t t)) self.slots
+      hash_mod in
   hashMap_contains_key_in_list t key l
 
-(** [hashmap::HashMap::{0}::get_in_list]: loop 0: forward function *)
+(** [hashmap::{hashmap::HashMap<T>}::get_in_list]: loop 0: forward function *)
 let rec hashMap_get_in_list_loop
   (t : Type0) (key : usize) (ls : list_t t) :
   Tot (result t) (decreases (hashMap_get_in_list_loop_decreases t key ls))
@@ -278,22 +276,22 @@ let rec hashMap_get_in_list_loop
   | List_Nil -> Fail Failure
   end
 
-(** [hashmap::HashMap::{0}::get_in_list]: forward function *)
+(** [hashmap::{hashmap::HashMap<T>}::get_in_list]: forward function *)
 let hashMap_get_in_list (t : Type0) (key : usize) (ls : list_t t) : result t =
   hashMap_get_in_list_loop t key ls
 
-(** [hashmap::HashMap::{0}::get]: forward function *)
+(** [hashmap::{hashmap::HashMap<T>}::get]: forward function *)
 let hashMap_get (t : Type0) (self : hashMap_t t) (key : usize) : result t =
   let* hash = hash_key key in
   let i = alloc_vec_Vec_len (list_t t) self.slots in
   let* hash_mod = usize_rem hash i in
   let* l =
     alloc_vec_Vec_index (list_t t) usize
-      (core_slice_index_usize_coresliceindexSliceIndexInst (list_t t))
-      self.slots hash_mod in
+      (core_slice_index_SliceIndexUsizeSliceTInst (list_t t)) self.slots
+      hash_mod in
   hashMap_get_in_list t key l
 
-(** [hashmap::HashMap::{0}::get_mut_in_list]: loop 0: forward function *)
+(** [hashmap::{hashmap::HashMap<T>}::get_mut_in_list]: loop 0: forward function *)
 let rec hashMap_get_mut_in_list_loop
   (t : Type0) (ls : list_t t) (key : usize) :
   Tot (result t) (decreases (hashMap_get_mut_in_list_loop_decreases t ls key))
@@ -304,12 +302,12 @@ let rec hashMap_get_mut_in_list_loop
   | List_Nil -> Fail Failure
   end
 
-(** [hashmap::HashMap::{0}::get_mut_in_list]: forward function *)
+(** [hashmap::{hashmap::HashMap<T>}::get_mut_in_list]: forward function *)
 let hashMap_get_mut_in_list
   (t : Type0) (ls : list_t t) (key : usize) : result t =
   hashMap_get_mut_in_list_loop t ls key
 
-(** [hashmap::HashMap::{0}::get_mut_in_list]: loop 0: backward function 0 *)
+(** [hashmap::{hashmap::HashMap<T>}::get_mut_in_list]: loop 0: backward function 0 *)
 let rec hashMap_get_mut_in_list_loop_back
   (t : Type0) (ls : list_t t) (key : usize) (ret : t) :
   Tot (result (list_t t))
@@ -325,23 +323,23 @@ let rec hashMap_get_mut_in_list_loop_back
   | List_Nil -> Fail Failure
   end
 
-(** [hashmap::HashMap::{0}::get_mut_in_list]: backward function 0 *)
+(** [hashmap::{hashmap::HashMap<T>}::get_mut_in_list]: backward function 0 *)
 let hashMap_get_mut_in_list_back
   (t : Type0) (ls : list_t t) (key : usize) (ret : t) : result (list_t t) =
   hashMap_get_mut_in_list_loop_back t ls key ret
 
-(** [hashmap::HashMap::{0}::get_mut]: forward function *)
+(** [hashmap::{hashmap::HashMap<T>}::get_mut]: forward function *)
 let hashMap_get_mut (t : Type0) (self : hashMap_t t) (key : usize) : result t =
   let* hash = hash_key key in
   let i = alloc_vec_Vec_len (list_t t) self.slots in
   let* hash_mod = usize_rem hash i in
   let* l =
     alloc_vec_Vec_index_mut (list_t t) usize
-      (core_slice_index_usize_coresliceindexSliceIndexInst (list_t t))
-      self.slots hash_mod in
+      (core_slice_index_SliceIndexUsizeSliceTInst (list_t t)) self.slots
+      hash_mod in
   hashMap_get_mut_in_list t l key
 
-(** [hashmap::HashMap::{0}::get_mut]: backward function 0 *)
+(** [hashmap::{hashmap::HashMap<T>}::get_mut]: backward function 0 *)
 let hashMap_get_mut_back
   (t : Type0) (self : hashMap_t t) (key : usize) (ret : t) :
   result (hashMap_t t)
@@ -351,16 +349,16 @@ let hashMap_get_mut_back
   let* hash_mod = usize_rem hash i in
   let* l =
     alloc_vec_Vec_index_mut (list_t t) usize
-      (core_slice_index_usize_coresliceindexSliceIndexInst (list_t t))
-      self.slots hash_mod in
+      (core_slice_index_SliceIndexUsizeSliceTInst (list_t t)) self.slots
+      hash_mod in
   let* l0 = hashMap_get_mut_in_list_back t l key ret in
   let* v =
     alloc_vec_Vec_index_mut_back (list_t t) usize
-      (core_slice_index_usize_coresliceindexSliceIndexInst (list_t t))
-      self.slots hash_mod l0 in
+      (core_slice_index_SliceIndexUsizeSliceTInst (list_t t)) self.slots
+      hash_mod l0 in
   Return { self with slots = v }
 
-(** [hashmap::HashMap::{0}::remove_from_list]: loop 0: forward function *)
+(** [hashmap::{hashmap::HashMap<T>}::remove_from_list]: loop 0: forward function *)
 let rec hashMap_remove_from_list_loop
   (t : Type0) (key : usize) (ls : list_t t) :
   Tot (result (option t))
@@ -379,12 +377,12 @@ let rec hashMap_remove_from_list_loop
   | List_Nil -> Return None
   end
 
-(** [hashmap::HashMap::{0}::remove_from_list]: forward function *)
+(** [hashmap::{hashmap::HashMap<T>}::remove_from_list]: forward function *)
 let hashMap_remove_from_list
   (t : Type0) (key : usize) (ls : list_t t) : result (option t) =
   hashMap_remove_from_list_loop t key ls
 
-(** [hashmap::HashMap::{0}::remove_from_list]: loop 0: backward function 1 *)
+(** [hashmap::{hashmap::HashMap<T>}::remove_from_list]: loop 0: backward function 1 *)
 let rec hashMap_remove_from_list_loop_back
   (t : Type0) (key : usize) (ls : list_t t) :
   Tot (result (list_t t))
@@ -405,12 +403,12 @@ let rec hashMap_remove_from_list_loop_back
   | List_Nil -> Return List_Nil
   end
 
-(** [hashmap::HashMap::{0}::remove_from_list]: backward function 1 *)
+(** [hashmap::{hashmap::HashMap<T>}::remove_from_list]: backward function 1 *)
 let hashMap_remove_from_list_back
   (t : Type0) (key : usize) (ls : list_t t) : result (list_t t) =
   hashMap_remove_from_list_loop_back t key ls
 
-(** [hashmap::HashMap::{0}::remove]: forward function *)
+(** [hashmap::{hashmap::HashMap<T>}::remove]: forward function *)
 let hashMap_remove
   (t : Type0) (self : hashMap_t t) (key : usize) : result (option t) =
   let* hash = hash_key key in
@@ -418,15 +416,15 @@ let hashMap_remove
   let* hash_mod = usize_rem hash i in
   let* l =
     alloc_vec_Vec_index_mut (list_t t) usize
-      (core_slice_index_usize_coresliceindexSliceIndexInst (list_t t))
-      self.slots hash_mod in
+      (core_slice_index_SliceIndexUsizeSliceTInst (list_t t)) self.slots
+      hash_mod in
   let* x = hashMap_remove_from_list t key l in
   begin match x with
   | None -> Return None
   | Some x0 -> let* _ = usize_sub self.num_entries 1 in Return (Some x0)
   end
 
-(** [hashmap::HashMap::{0}::remove]: backward function 0 *)
+(** [hashmap::{hashmap::HashMap<T>}::remove]: backward function 0 *)
 let hashMap_remove_back
   (t : Type0) (self : hashMap_t t) (key : usize) : result (hashMap_t t) =
   let* hash = hash_key key in
@@ -434,24 +432,24 @@ let hashMap_remove_back
   let* hash_mod = usize_rem hash i in
   let* l =
     alloc_vec_Vec_index_mut (list_t t) usize
-      (core_slice_index_usize_coresliceindexSliceIndexInst (list_t t))
-      self.slots hash_mod in
+      (core_slice_index_SliceIndexUsizeSliceTInst (list_t t)) self.slots
+      hash_mod in
   let* x = hashMap_remove_from_list t key l in
   begin match x with
   | None ->
     let* l0 = hashMap_remove_from_list_back t key l in
     let* v =
       alloc_vec_Vec_index_mut_back (list_t t) usize
-        (core_slice_index_usize_coresliceindexSliceIndexInst (list_t t))
-        self.slots hash_mod l0 in
+        (core_slice_index_SliceIndexUsizeSliceTInst (list_t t)) self.slots
+        hash_mod l0 in
     Return { self with slots = v }
   | Some x0 ->
     let* i0 = usize_sub self.num_entries 1 in
     let* l0 = hashMap_remove_from_list_back t key l in
     let* v =
       alloc_vec_Vec_index_mut_back (list_t t) usize
-        (core_slice_index_usize_coresliceindexSliceIndexInst (list_t t))
-        self.slots hash_mod l0 in
+        (core_slice_index_SliceIndexUsizeSliceTInst (list_t t)) self.slots
+        hash_mod l0 in
     Return { self with num_entries = i0; slots = v }
   end
 
