tests/fstar/hashmap_on_disk/HashmapMain.Clauses.Template.fst
@@ -6,56 +6,56 @@ open HashmapMain.Types
 
 #set-options "--z3rlimit 50 --fuel 1 --ifuel 1"
 
-(** [hashmap_main::hashmap::HashMap::{0}::allocate_slots]: decreases clause *)
+(** [hashmap_main::hashmap::{hashmap_main::hashmap::HashMap<T>}::allocate_slots]: decreases clause *)
 unfold
 let hashmap_HashMap_allocate_slots_loop_decreases (t : Type0)
   (slots : alloc_vec_Vec (hashmap_List_t t)) (n : usize) : nat =
   admit ()
 
-(** [hashmap_main::hashmap::HashMap::{0}::clear]: decreases clause *)
+(** [hashmap_main::hashmap::{hashmap_main::hashmap::HashMap<T>}::clear]: decreases clause *)
 unfold
 let hashmap_HashMap_clear_loop_decreases (t : Type0)
   (slots : alloc_vec_Vec (hashmap_List_t t)) (i : usize) : nat =
   admit ()
 
-(** [hashmap_main::hashmap::HashMap::{0}::insert_in_list]: decreases clause *)
+(** [hashmap_main::hashmap::{hashmap_main::hashmap::HashMap<T>}::insert_in_list]: decreases clause *)
 unfold
 let hashmap_HashMap_insert_in_list_loop_decreases (t : Type0) (key : usize)
   (value : t) (ls : hashmap_List_t t) : nat =
   admit ()
 
-(** [hashmap_main::hashmap::HashMap::{0}::move_elements_from_list]: decreases clause *)
+(** [hashmap_main::hashmap::{hashmap_main::hashmap::HashMap<T>}::move_elements_from_list]: decreases clause *)
 unfold
 let hashmap_HashMap_move_elements_from_list_loop_decreases (t : Type0)
   (ntable : hashmap_HashMap_t t) (ls : hashmap_List_t t) : nat =
   admit ()
 
-(** [hashmap_main::hashmap::HashMap::{0}::move_elements]: decreases clause *)
+(** [hashmap_main::hashmap::{hashmap_main::hashmap::HashMap<T>}::move_elements]: decreases clause *)
 unfold
 let hashmap_HashMap_move_elements_loop_decreases (t : Type0)
   (ntable : hashmap_HashMap_t t) (slots : alloc_vec_Vec (hashmap_List_t t))
   (i : usize) : nat =
   admit ()
 
-(** [hashmap_main::hashmap::HashMap::{0}::contains_key_in_list]: decreases clause *)
+(** [hashmap_main::hashmap::{hashmap_main::hashmap::HashMap<T>}::contains_key_in_list]: decreases clause *)
 unfold
 let hashmap_HashMap_contains_key_in_list_loop_decreases (t : Type0)
   (key : usize) (ls : hashmap_List_t t) : nat =
   admit ()
 
-(** [hashmap_main::hashmap::HashMap::{0}::get_in_list]: decreases clause *)
+(** [hashmap_main::hashmap::{hashmap_main::hashmap::HashMap<T>}::get_in_list]: decreases clause *)
 unfold
 let hashmap_HashMap_get_in_list_loop_decreases (t : Type0) (key : usize)
   (ls : hashmap_List_t t) : nat =
   admit ()
 
-(** [hashmap_main::hashmap::HashMap::{0}::get_mut_in_list]: decreases clause *)
+(** [hashmap_main::hashmap::{hashmap_main::hashmap::HashMap<T>}::get_mut_in_list]: decreases clause *)
 unfold
 let hashmap_HashMap_get_mut_in_list_loop_decreases (t : Type0)
   (ls : hashmap_List_t t) (key : usize) : nat =
   admit ()
 
-(** [hashmap_main::hashmap::HashMap::{0}::remove_from_list]: decreases clause *)
+(** [hashmap_main::hashmap::{hashmap_main::hashmap::HashMap<T>}::remove_from_list]: decreases clause *)
 unfold
 let hashmap_HashMap_remove_from_list_loop_decreases (t : Type0) (key : usize)
   (ls : hashmap_List_t t) : nat =
