tests/fstar/misc/External.Opaque.fsti
@@ -17,11 +17,11 @@ val core_mem_swap_back0
 val core_mem_swap_back1
   (t : Type0) : t -> t -> state -> state -> result (state & t)
 
-(** [core::num::nonzero::NonZeroU32::{14}::new]: forward function *)
+(** [core::num::nonzero::{core::num::nonzero::NonZeroU32#14}::new]: forward function *)
 val core_num_nonzero_NonZeroU32_new
   : u32 -> state -> result (state & (option core_num_nonzero_NonZeroU32_t))
 
-(** [core::option::Option::{0}::unwrap]: forward function *)
+(** [core::option::{core::option::Option<T>}::unwrap]: forward function *)
 val core_option_Option_unwrap
   (t : Type0) : option t -> state -> result (state & t)
 
